addressing #2500

examples/MutableMap/MutableMapDafny.dfy
@@ -4,16 +4,58 @@
 *******************************************************************************/
 
 // RUN: %verify "%s"
-
-include "MutableMapTrait.dfy"
    
 /**
   *  Implements mutable maps in Dafny to guard against inconsistent specifications.
   *  Only exists to verify feasability; not meant for actual usage.
   */
 module {:options "-functionSyntax:4"} MutableMapDafny {
-  import opened MutableMapTrait
-  
+  /**
+    *  NOTE: Only here because of #2500; once resolved import "MutableMapTrait.dfy".
+    */
+  trait {:termination false} MutableMapTrait<K(==),V(==)> {
+    function content(): map<K, V>
+      reads this
+
+    method Put(k: K, v: V)
+      modifies this
+      ensures this.content() == old(this.content())[k := v]   
+      ensures k in old(this.content()).Keys ==> this.content().Values + {old(this.content())[k]} == old(this.content()).Values + {v}
+      ensures k !in old(this.content()).Keys ==> this.content().Values == old(this.content()).Values + {v}
+
+    function Keys(): (keys: set<K>)
+      reads this
+      ensures keys == this.content().Keys
+
+    predicate HasKey(k: K)
+      reads this
+      ensures HasKey(k) <==> k in this.content().Keys
+
+    function Values(): (values: set<V>)
+      reads this
+      ensures values == this.content().Values
+
+    function Items(): (items: set<(K,V)>)
+      reads this
+      ensures items == this.content().Items
+      ensures items == set k | k in this.content().Keys :: (k, this.content()[k])
+
+    function Select(k: K): (v: V)
+      reads this
+      requires this.HasKey(k)
+      ensures v in this.content().Values
+      ensures this.content()[k] == v
+
+    method Remove(k: K)
+      modifies this
+      ensures this.content() == old(this.content()) - {k}
+      ensures k in old(this.content()).Keys ==> this.content().Values + {old(this.content())[k]} == old(this.content()).Values
+ 
+    function Size(): (size: int)
+      reads this
+      ensures size == |this.content().Items|
+  }
+
   class MutableMapDafny<K(==),V(==)> extends MutableMapTrait<K,V> {
     var m: map<K,V>
 
