src/MutableMap/MutableMap.dfy
@@ -5,7 +5,6 @@
 
 // RUN: %verify "%s"
 
-include "../../examples/MutableMap/MutableMapTrait.dfy"
 include "../../src/Wrappers.dfy"
 
 /**
@@ -13,8 +12,54 @@ include "../../src/Wrappers.dfy"
   */
 
 module {:extern "DafnyLibraries"} {:options "-functionSyntax:4"} DafnyLibraries {
-  import opened MutableMapTrait
   import opened Wrappers
+
+  /**
+  *  NOTE: Only here because of #2500; once resolved import "../../examples/MutableMap/
+  *  MutableMapTrait.dfy".
+  */
+  trait {:termination false} MutableMapTrait<K(==),V(==)> {
+    function content(): map<K, V>
+      reads this
+
+    method Put(k: K, v: V)
+      modifies this
+      ensures this.content() == old(this.content())[k := v]   
+      ensures k in old(this.content()).Keys ==> this.content().Values + {old(this.content())[k]} == old(this.content()).Values + {v}
+      ensures k !in old(this.content()).Keys ==> this.content().Values == old(this.content()).Values + {v}
+
+    function Keys(): (keys: set<K>)
+      reads this
+      ensures keys == this.content().Keys
+
+    predicate HasKey(k: K)
+      reads this
+      ensures HasKey(k) <==> k in this.content().Keys
+
+    function Values(): (values: set<V>)
+      reads this
+      ensures values == this.content().Values
+
+    function Items(): (items: set<(K,V)>)
+      reads this
+      ensures items == this.content().Items
+      ensures items == set k | k in this.content().Keys :: (k, this.content()[k])
+
+    function Select(k: K): (v: V)
+      reads this
+      requires this.HasKey(k)
+      ensures v in this.content().Values
+      ensures this.content()[k] == v
+
+    method Remove(k: K)
+      modifies this
+      ensures this.content() == old(this.content()) - {k}
+      ensures k in old(this.content()).Keys ==> this.content().Values + {old(this.content())[k]} == old(this.content()).Values
+ 
+    function Size(): (size: int)
+      reads this
+      ensures size == |this.content().Items|
+  }
 
   class {:extern} MutableMap<K(==),V(==)> extends MutableMapTrait<K,V> {
     constructor {:extern} ()
